hol/multiequation_systemScript.sml
@@ -213,24 +213,73 @@ first_x_assum (qspec_then `\n. if EVEN n then x else y` mp_tac) >>
 srw_tac [][] >>
 Cases_on `EVEN n` >> fsrw_tac [][arithmeticTheory.EVEN] );
 
+val antisymmetric_RINTER = Q.store_thm(
+"antisymmetric_RINTER",
+`antisymmetric R ⇒ antisymmetric (R RINTER R')`,
+srw_tac [][antisymmetric_def,RINTER]);
+
+val transitive_RINTER = Q.store_thm(
+"transitive_RINTER",
+`transitive R1 ∧ transitive R2 ⇒ transitive (R1 RINTER R2)`,
+srw_tac [SATISFY_ss][transitive_def,RINTER]);
+
+val bounded_Order_has_greatest = Q.store_thm(
+"bounded_Order_has_greatest",
+`∀s. FINITE s ⇒ ∀R. Order R ∧ (!x y. R x y ⇒ x ∈ s ∧ y ∈ s) ∧ s ≠ {} ⇒ ∃e. e ∈ s ∧ ∀x. x ∈ s ∧ x ≠ e ⇒ ¬ R e x`,
+ho_match_mp_tac FINITE_INDUCT >>
+srw_tac [DNF_ss][] >>
+Cases_on `s = {}` >> srw_tac [][] >>
+Cases_on `!x. x ∈ s ∧ x ≠ e ⇒ ¬ R e x` >> srw_tac [][] >>
+fsrw_tac [][] >>
+Q.ABBREV_TAC `RR = R RINTER (\x y. x ≠ e ∧ y ≠ e)` >>
+`Order RR` by (
+  fsrw_tac [][Abbr`RR`,Order,antisymmetric_RINTER] >>
+  match_mp_tac transitive_RINTER >>
+  srw_tac [][] >>
+  srw_tac [][transitive_def]) >>
+`∀x y. RR x y ⇒ x ∈ s ∧ y ∈ s` by (
+  srw_tac [][Abbr`RR`,FORALL_PROD,RINTER] >>
+  PROVE_TAC [] ) >>
+fsrw_tac [DNF_ss][] >>
+first_x_assum (qspec_then `RR` mp_tac) >>
+srw_tac [SATISFY_ss][] >>
+qmatch_assum_rename_tac `!x. x ∈ s ∧ x ≠ xold ⇒ ¬RR xold x` [] >>
+Cases_on `x = xold` >- (
+  qexists_tac `x` >> srw_tac [][] >- (
+    PROVE_TAC [Order,antisymmetric_def] ) >>
+  fsrw_tac [][Abbr`RR`,RINTER] >>
+  PROVE_TAC [Order,antisymmetric_def] ) >>
+Cases_on `R xold x` >- (
+  qexists_tac `x` >> srw_tac [][] >- (
+    PROVE_TAC [Order,antisymmetric_def]) >>
+  fsrw_tac [][Abbr`RR`,RINTER] >>
+  PROVE_TAC [Order,antisymmetric_def] ) >>
+qexists_tac `xold` >> srw_tac [][] >- (
+  spose_not_then strip_assume_tac >>
+  PROVE_TAC [transitive_def,Order] ) >>
+fsrw_tac [][Abbr`RR`,RINTER] >>
+PROVE_TAC []);
+
 val top_meq_exists = Q.store_thm( (* Corollary to Theorem 3.3 *)
 "top_meq_exists",
-`RES_FORALL meqs wfm ∧ pairwise (RC (inv_image DISJOINT FST)) meqs ∧
+`FINITE meqs ∧ RES_FORALL meqs wfm ∧ pairwise (RC (inv_image DISJOINT FST)) meqs ∧
  meqs_unifier meqs ≠ {} ∧ meqs ≠ {} ⇒
  ∃meq. meq ∈ meqs ∧
        ∀meq'. meq' ∈ meqs ∧ meq' ≠ meq ⇒
               DISJOINT (FST meq) (FST meq') ∧
-              DISJOINT (FST meq) (BIGUNION (IMAGE vars (SET_OF_BAG (SND meq))))`,
+              DISJOINT (FST meq) (bag_vars (SND meq'))`,
 strip_tac >> imp_res_tac WF_meqR >>
-fsrw_tac [DNF_ss][RES_FORALL_THM,pairwise_def,RC_DEF,inv_image_def,IN_DISJOINT,FORALL_PROD] >>
-fsrw_tac [][WF_DEF] >>
-first_x_assum (qspec_then `\meq. meq ∈ meqs` mp_tac) >>
-fsrw_tac [DNF_ss,SATISFY_ss][GSYM pred_setTheory.MEMBER_NOT_EMPTY] >>
-srw_tac [][] >>
-qexists_tac `min` >>
-fsrw_tac [][meqR_def] >>
-Cases_on `min` >>
-srw_tac [][] >> fsrw_tac [][] >>
-PROVE_TAC [FST]);
+`Order (meqR meqs)^+` by PROVE_TAC [transitive_WF_imp_StrongOrder,WF_TC,TC_TRANSITIVE,Order,StrongOrder] >>
+`!x y. (meqR meqs)^+ x y ⇒ x ∈ meqs ∧ y ∈ meqs` by (
+  ho_match_mp_tac TC_lifts_transitive_relations >>
+  srw_tac [][meqR_def,transitive_def] ) >>
+`?max. max ∈ meqs ∧ ∀meq. meq ∈ meqs ∧ meq ≠ max ⇒ ¬ (meqR meqs)^+ max meq` by (
+  match_mp_tac (MP_CANON bounded_Order_has_greatest) >>
+  srw_tac [SATISFY_ss][] ) >>
+`!meq. meq ∈ meqs ∧ meq ≠ max ⇒ ¬ meqR meqs max meq` by PROVE_TAC [TC_SUBSET] >>
+qexists_tac `max` >>
+Cases_on `max` >>
+fsrw_tac [][IN_DISJOINT,pairwise_def,RC_DEF,inv_image_def,FORALL_PROD,bag_vars_def,meqR_def] >>
+PROVE_TAC []);
 
 val _ = export_theory ()
